examples/cms/LightModel.v
@@ -1,0 +1,413 @@
+Require Import Coq.ZArith.BinInt.
+Require Import Coq.Program.Program.
+Require Poulet4.Utils.Utils.
+Require Import ProD3.core.Coqlib.
+Require Import ProD3.examples.sbf.Utils.
+Require Import ProD3.examples.cms.AbsModel.
+Require Import Hammer.Plugin.Hammer.
+Import ListNotations.
+Open Scope Z_scope.
+Open Scope program_scope.
+
+Section LightModel.
+
+Context {header_type : Set}.
+Context (num_frames num_rows num_slots frame_time : Z).
+Hypothesis H_num_slots : 0 < num_slots.
+Hypothesis H_num_rows : 0 < num_rows.
+Hypothesis H_num_frames : 1 < num_frames.
+Context (hashes : list (header_type -> Z)).
+Hypothesis H_Zlength_hashes : Zlength hashes = num_rows.
+Hypothesis H_hashes : Forall (fun hash => forall h, 0 <= hash h < num_slots) hashes.
+
+Context (tick_time : Z).
+Hypothesis (H_tick_time : 0 < tick_time).
+
+Hypothesis (H_frame_time : 0 < frame_time).
+Hypothesis (H_tick_time_div : (tick_time * 2 | frame_time)).
+
+Definition filter := option (@cms header_type).
+
+Notation abs_insert := (@cms_insert header_type num_frames num_slots frame_time tick_time).
+Notation abs_query := (@cms_query header_type num_frames num_slots frame_time hashes tick_time).
+Notation abs_clear := (@cms_clear header_type num_frames num_slots frame_time tick_time).
+Notation abs_refresh := (@cms_refresh header_type num_frames num_slots frame_time tick_time).
+
+(* The time of guaranteed query, e.g. 59s. *)
+Definition T := frame_time * (num_frames - 2).
+
+(* The maximum time interval between consecutive packets, e.g. 112us. *)
+Definition Tc := frame_time / num_slots.
+
+(* This should be provable *)
+Lemma Tc_mul_num_slots_le_frame_time : Tc * num_slots <= frame_time.
+Proof. unfold Tc. rewrite Z.mul_comm. apply Z.mul_div_le. assumption. Qed.
+(* This seems NOT provable. *)
+Axiom Tc_le_tick_time : Tc <= tick_time.
+
+Lemma Tc_le_frame_time : Tc <= frame_time.
+Proof.
+  unfold Tc. apply Z.div_le_upper_bound; auto.
+  rewrite Z.mul_comm. apply Z.le_mul_diag_r; lia.
+Qed.
+
+Axiom H_Tc : 0 < Tc.
+(* Lemma Tc_le_T : Tc <= T.
+Admitted. *)
+
+Definition cms_insert (f : filter) (th : Z * header_type) : filter :=
+  match f with
+  | Some f => abs_insert f th
+  | None => None
+  end.
+
+Definition cms_query (f : filter) '((t, h) : Z * header_type) : option Z :=
+  match f with
+  | Some (mk_cms window_hi last_timestamp num_clears normal_frames) =>
+      if last_timestamp <=? t then
+        let num_invalid_frames := Z.min (Z.max ((t - window_hi) / frame_time + 1) 0) (num_frames - 1) in
+        let valid_frames := sublist num_invalid_frames (num_frames - 1) normal_frames in
+        let res := Zsum (map (fun hs => list_min (map (fun hash => Zsum (map (Z.b2z ∘ Z.eqb (hash h) ∘ hash) hs)) hashes)) valid_frames) in
+        Some res
+      else
+        None
+  | None => None
+  end.
+
+Definition cms_clear (f : filter) (t : Z) : filter :=
+  match f with
+  | Some f =>
+      abs_clear f t
+  | None => None
+  end.
+
+(* Axiom cms_empty : filter. *)
+
+Definition weak_cms_inv (f : filter) : Prop :=
+  match f with
+  | Some (mk_cms window_hi last_timestamp num_clears normal_frames) =>
+      window_hi - frame_time <= last_timestamp < window_hi /\
+      Zlength normal_frames = num_frames - 1
+  | None => False
+  end.
+
+Definition cms_inv (f : filter) : Prop :=
+  match f with
+  | Some (mk_cms window_hi last_timestamp num_clears normal_frames) =>
+      last_timestamp < window_hi /\
+      (window_hi - 1 - last_timestamp) / Tc + num_clears >= num_slots /\
+      Zlength normal_frames = num_frames - 1
+  | None => False
+  end.
+
+Definition ok_until (f : filter) (t : Z) : Prop :=
+  (* cms_inv f /\ *)
+  match f with
+  | Some (mk_cms window_hi last_timestamp num_clears normal_frames) =>
+      0 <= t - last_timestamp <= Tc /\ cms_inv f
+        (* last_timestamp < window_hi /\
+        (window_hi - 1 - last_timestamp) / Tc + num_clears >= num_slots *)
+  | None => False
+  end.
+
+Definition weak_cms_inv1 (f : filter) (new_timestamp : Z) : Prop :=
+  match f with
+  | Some (mk_cms window_hi last_timestamp num_clears normal_frames) =>
+      window_hi - frame_time <= new_timestamp < window_hi /\
+      Zlength normal_frames = num_frames - 1
+  | None => False
+  end.
+
+Definition cms_inv1 (f : filter) (new_timestamp : Z) : Prop :=
+  match f with
+  | Some (mk_cms window_hi last_timestamp num_clears normal_frames) =>
+      new_timestamp < window_hi /\
+      (window_hi - 1 - new_timestamp) / Tc + (num_clears + 1) >= num_slots /\
+      Zlength normal_frames = num_frames - 1
+  | None => False
+  end.
+
+Definition ok_until1 (f : filter) (new_timestamp : Z) (t : Z) : Prop :=
+  match f with
+  | Some (mk_cms window_hi _ num_clears normal_frames) =>
+      0 <= t - new_timestamp <= Tc /\ cms_inv1 f new_timestamp
+        (* new_timestamp < window_hi /\
+        (window_hi - 1 - new_timestamp) / Tc + (num_clears + 1) >= num_slots *)
+  | None => False
+  end.
+
+Lemma weak_cms_inv1_abs_refresh : forall f t,
+  weak_cms_inv (Some f) ->
+  match abs_refresh f t with
+  | Some f =>
+      weak_cms_inv1 (Some f) t
+  | None => True
+  end.
+Proof.
+  intros.
+  unfold weak_cms_inv, weak_cms_inv1 in *.
+  destruct f.
+  unfold abs_refresh.
+  destruct (last_timestamp <=? t) eqn:?H; only 2 : simpl; auto.
+  destruct (t <=? last_timestamp + tick_time) eqn:?H; only 2 : simpl; auto.
+  simpl andb. cbn match.
+  destruct (t >=? window_hi) eqn:?H.
+  - destruct (num_clears >=? num_slots); only 2 : auto.
+    split.
+    + assert (tick_time <= frame_time). {
+        destruct H_tick_time_div as [z ?]. subst.
+        replace (z * (tick_time * 2)) with (tick_time * (2 * z)) by lia.
+        apply Z.le_mul_diag_r; lia. } lia.
+    + list_solve.
+  - lia.
+Qed.
+
+(* This lemma shows cms_query (cms_clear ..) is equal to abs_query. *)
+Lemma abs_query_pattern_ok : forall f t h res,
+  weak_cms_inv (Some f) ->
+  cms_query (cms_clear (Some f) t) (t, h) = Some res ->
+  exists f', abs_query f (t, h) = Some (f', res).
+Proof.
+  intros * ?H H_cms_query.
+  unfold cms_clear, cms_query, abs_clear, abs_query in *.
+  pose proof (weak_cms_inv1_abs_refresh f t ltac:(auto)).
+  destruct (abs_refresh f t) as [[window_hi last_timestamp num_clears normal_frames] | ].
+    2 : inv H_cms_query.
+  unfold weak_cms_inv1 in *.
+  assert ((t - window_hi) / frame_time + 1 = 0). {
+    rewrite <- Zdiv.Z_div_plus by lia.
+    apply Z.div_small; lia.
+  }
+  destruct (t <=? t) eqn:?H.
+    2 : inv H_cms_query.
+  eexists. f_equal. f_equal.
+  inv H_cms_query.
+  f_equal. list_solve.
+Qed.
+
+Lemma ok_refresh : forall f t t',
+  t <= t' <= t + Tc ->
+  ok_until (Some f) t ->
+  ok_until1 (abs_refresh f t) t t'.
+Proof.
+  intros * H_t' H_ok_until.
+  destruct f as [window_hi last_timestamp num_clears normal_frames].
+  simpl in *.
+  replace (last_timestamp <=? t) with true by lia.
+  replace (t <=? last_timestamp + tick_time) with true by (pose Tc_le_tick_time; lia).
+  destruct (t >=? window_hi) eqn:?H.
+  - assert (0 <= window_hi - 1 - last_timestamp < Tc) by (pose Tc_le_tick_time; lia).
+    rewrite Z.div_small in H_ok_until by lia.
+    replace (num_clears >=? num_slots) with true by lia.
+    simpl.
+    split; only 1 : lia.
+    split; only 1 : (pose Tc_le_frame_time; lia).
+    split; only 2 : list_solve.
+    pose proof Tc_mul_num_slots_le_frame_time.
+    assert (window_hi - t >= 1 - Tc) by lia.
+    assert ((window_hi + frame_time - 1 - t) / Tc + 1 >= frame_time / Tc). {
+      replace (frame_time / Tc) with ((frame_time - Tc) / Tc + 1).
+      - apply Z.le_ge, Z.add_le_mono_r, Z.ge_le, Zdiv.Z_div_ge; lia.
+      - rewrite <- Z.add_opp_r. change (- Tc) with ((- 1) * Tc).
+        rewrite Z.div_add; lia. }
+    apply Zorder.Zge_trans with (frame_time / Tc); auto.
+    apply Z.div_le_mono with (c := Tc) in H1. 2: lia.
+    rewrite Z.mul_comm, Z.div_mul in H1; lia.
+  - simpl.
+    split; only 1 : lia.
+    split; only 1 : lia.
+    split; only 2 : lia.
+    assert ((window_hi - 1 - last_timestamp + (-1) * Tc) / Tc <= (window_hi - 1 - t) / Tc). {
+      apply Z.div_le_mono. 2 : lia.
+      apply H_Tc.
+    }
+    rewrite Zdiv.Z_div_plus in * by (pose proof H_Tc; lia).
+    lia.
+Qed.
+
+Lemma query_clear : forall f t t' h,
+  t <= t' ->
+  ok_until f t ->
+  cms_query f (t', h) = cms_query (cms_clear f t) (t', h).
+Proof.
+  intros * H_t' H_ok_until.
+  destruct f. 2 : inv H_ok_until.
+  destruct c as [window_hi last_timestamp num_clears normal_frames].
+  unfold cms_clear, abs_clear, abs_refresh, ok_until, cms_inv in *.
+  replace (last_timestamp <=? t) with true by lia.
+  replace (t <=? last_timestamp + tick_time) with true by (pose Tc_le_tick_time; lia).
+  destruct (t >=? window_hi) eqn:?H.
+  - assert (0 <= window_hi - 1 - last_timestamp < Tc) by (pose Tc_le_tick_time; lia).
+    rewrite Z.div_small in H_ok_until by lia.
+    replace (num_clears >=? num_slots) with true by lia.
+    cbn -[cms_query sublist].
+    unfold cms_query.
+    replace (last_timestamp <=? t') with true by lia.
+    replace (t <=? t') with true by lia.
+    remember (Z.max ((t' - window_hi) / frame_time + 1) 0) as k eqn:?H.
+    assert ((t' - window_hi) / frame_time >= 0). {
+      apply Zdiv.Z_div_ge0; lia.
+    }
+    replace (Z.max ((t' - (window_hi + frame_time)) / frame_time + 1) 0) with (k - 1). 2 : {
+      replace (t' - (window_hi + frame_time)) with (t' - window_hi + (-1) * frame_time) by lia.
+      rewrite Z.div_add by lia.
+      lia.
+    }
+    destruct (k - 1 >=? (num_frames - 1)) eqn:?H.
+    { replace (sublist (Z.min k (num_frames - 1)) (num_frames - 1) _)
+        with (@nil (list header_type)) by list_solve.
+      replace (sublist (Z.min (k - 1) (num_frames - 1)) (num_frames - 1) _)
+        with (@nil (list header_type)) by list_solve.
+      auto.
+    }
+    destruct (k >=? (num_frames - 1)) eqn:?H.
+    { replace (sublist (Z.min k (num_frames - 1)) (num_frames - 1) _)
+        with (@nil (list header_type)) by list_solve.
+      replace (sublist (Z.min (k - 1) (num_frames - 1)) (num_frames - 1) _)
+        with ([@nil header_type]) by list_solve.
+      destruct hashes as [ | hash0 hashes']. 1 : list_solve. unfold Zsum. simpl.
+      clear. induction hashes'; simpl; auto.
+    }
+    replace (sublist (Z.min k (num_frames - 1)) (num_frames - 1) _)
+        with (sublist k (num_frames - 1) normal_frames) by list_solve.
+    replace (sublist (Z.min (k - 1) (num_frames - 1)) (num_frames - 1) _)
+      with (sublist k (num_frames - 1) normal_frames ++ [[]]) by list_solve.
+    rewrite map_app. simpl.
+    replace (list_min (map (fun _ : header_type -> Z => Zsum []) hashes)) with 0.
+    2: { unfold Zsum. simpl. destruct hashes as [ | hash0 hashes']. 1 : list_solve.
+         simpl. clear. induction hashes'; simpl; auto. }
+    rewrite Zsum_app. replace (Zsum [0]) with 0 by (unfold Zsum; now simpl).
+    rewrite Z.add_0_r. auto.
+  - simpl.
+    replace (last_timestamp <=? t') with true by lia.
+    replace (t <=? t') with true by lia.
+    auto.
+Qed.
+
+Lemma ok_until_query_some : forall f t h, ok_until f t -> exists k, cms_query f (t, h) = Some k.
+Proof.
+  intros f t h H_ok_until.
+  destruct f. 2: inv H_ok_until. red in H_ok_until. destruct c.
+  destruct H_ok_until as [[Ht _] _]. simpl.
+  destruct (last_timestamp <=? t) eqn:Hlt. 2: lia.
+  match goal with
+  | |- exists _, Some ?i = Some _ => exists i; reflexivity
+  end.
+Qed.
+
+Lemma query_insert_same : forall f t t' h k,
+  t <= t' <= t + T ->
+  ok_until f t ->
+  cms_query f (t', h) = Some k ->
+  cms_query (cms_insert f (t, h)) (t', h) = Some (k + 1).
+Proof.
+  intros f t t' h k Ht' H_ok_until H_cms_query.
+  assert (H_query_clear : cms_query (cms_clear f t) (t', h) = Some k). {
+    erewrite <- query_clear; eauto. lia.
+  }
+  clear H_cms_query.
+  unfold cms_clear, abs_clear, cms_insert, abs_insert in *.
+  destruct f. 2 : inv H_ok_until.
+  pose proof (H_ok_refresh := ok_refresh c t t ltac:(pose proof H_Tc; lia) ltac:(auto)).
+  destruct (abs_refresh c t) as [f' | ] in *. 2 : inv H_ok_refresh.
+  destruct f'.
+  unfold cms_query, ok_until1, cms_inv1 in *.
+  destruct (t <=? t') eqn:?H. 2 : inv H_query_clear.
+  injection H_query_clear; clear H_query_clear; intros H_query_clear. f_equal.
+  (*
+  assert ((t' - window_hi) / frame_time < num_frames - 2). {
+    apply Z.div_lt_upper_bound. 1 : lia.
+    fold T.
+    lia.
+  }
+  f_equal.
+  apply existsb_Znth_true with (i := num_frames - 2 - Z.max ((t' - window_hi) / frame_time + 1) 0).
+  { list_solve. }
+  rewrite forallb_fold_andb.
+  apply fold_andb_true; list_simplify; intros.
+  rewrite <- existsb_fold_orb.
+  list_simplify.
+  rewrite existsb_app.
+  simpl.
+  unfold compose.
+  replace (Znth i hashes h =? Znth i hashes h) with true by lia.
+  rewrite orbF.
+  rewrite orbT.
+  auto. *)
+
+Abort.
+
+(*
+
+Lemma query_insert_other : forall f t t' h h',
+  t <= t' ->
+  ok_until f t ->
+  cms_query f (t', h') = Some true ->
+  cms_query (cms_insert f (t, h)) (t', h') = Some true.
+Proof.
+  intros * H_t' H_ok_until H_cms_query.
+  assert (H_query_clear : cms_query (cms_clear f t) (t', h') = Some true). {
+    erewrite <- query_clear; eauto.
+  }
+  clear H_cms_query.
+  unfold cms_clear, abs_clear, cms_insert, abs_insert in *.
+  destruct f. 2 : inv H_ok_until.
+  pose proof (H_ok_refresh := ok_refresh f t t ltac:(pose proof H_Tc; lia) ltac:(auto)).
+  destruct (abs_refresh f t) as [f' | ] eqn:?H. 2 : inv H_query_clear.
+  destruct f' as [window_hi last_timestamp num_clears normal_frames].
+  unfold cms_query in *.
+  destruct (t <=? t') eqn:?H. 2 : inv H_query_clear.
+  injection H_query_clear; clear H_query_clear; intros H_query_clear. f_equal.
+  apply existsb_true_Znth in H_query_clear.
+  destruct H_query_clear as [i []].
+  assert (Zlength normal_frames = num_frames - 1). {
+    apply H_ok_refresh.
+  }
+  apply existsb_Znth_true with (i := i).
+  { list_solve. }
+  list_simplify.
+  rewrite e in H2.
+  clear -H2.
+  apply forallb_true_Znth in H2.
+  apply forallb_Znth_true.
+  list_simplify.
+  rewrite <- existsb_fold_orb in *.
+  rewrite existsb_app.
+  clear -H5; hauto lq: on.
+Qed.
+
+Lemma ok_insert : forall f t t' h,
+  t <= t' <= t + Tc ->
+  ok_until f t ->
+  ok_until (cms_insert f (t, h)) t'.
+Proof.
+  intros * H_t' H_ok_until.
+  destruct f. 2 : inv H_ok_until.
+  pose proof (H_ok_refresh := ok_refresh f t t' ltac:(auto) ltac:(auto)).
+  unfold cms_insert, abs_insert in *.
+  destruct (abs_refresh f t). 2 : inv H_ok_refresh.
+  destruct f0.
+  unfold ok_until, cms_inv.
+  rewrite Zlength_upd_Znth.
+  apply H_ok_refresh.
+Qed.
+
+Lemma ok_clear : forall f t t',
+  t <= t' <= t + Tc ->
+  ok_until f t ->
+  ok_until (cms_clear f t) t'.
+Proof.
+  intros * H_t' H_ok_until.
+  destruct f. 2 : inv H_ok_until.
+  pose proof (H_ok_refresh := ok_refresh f t t' ltac:(auto) ltac:(auto)).
+  unfold cms_clear, abs_clear in *.
+  destruct (abs_refresh f t). 2 : inv H_ok_refresh.
+  destruct f0. apply H_ok_refresh.
+Qed.
+
+(* Lemma ok_empty: forall t,
+  ok_until empty t. *)
+
+*)
+
+End LightModel.
